Prove responder as well, modulo some set-related admits.

nsl_dh.v
@@ -31,7 +31,7 @@ Definition dh_initiator : val := λ: "skA" "pkA" "pkB",
 
 Definition dh_responder : val := λ: "skB" "pkB",
   let: "b" := mknonce #() in
-  let: "gb" := texp (tgroup (tint #0)) in
+  let: "gb" := texp (tgroup (tint #0)) "b" in
   bind: "res" := responder send recv "skB" "pkB" "gb" in
   let: "pkA" := Fst "res" in
   let: "ga" := Snd "res" in
@@ -60,6 +60,78 @@ Definition nsl_dh_inv rl kA kB ga gb : iProp :=
     □ ∀ a, (pterm (TExp (TInt 0) [a; b]) → ▷ pterm a)
   end%I.
 
+Definition nsl_dh_pred k t : iProp :=
+  ∃ a k',
+    meta a (cryptoN.@"dh") k' ∧
+    (pterm (TKey Dec k) ∨ pterm (TKey Dec k')) ∧
+    ⌜t = TExp (TInt 0) [TNonce a]⌝.
+
+Lemma nsl_dh_predN k t : negb (is_exp t) → nsl_dh_pred k t -∗ False.
+Proof.
+iIntros (nexp); iDestruct 1 as (a k') "# (_ & _ & %contra)".
+by move: nexp contra; rewrite unlock; case: t.
+Qed.
+
+Lemma nsl_dh_predX1 a k k' :
+  meta a (cryptoN.@"dh") k' -∗
+  nsl_dh_pred k (TExp (TInt 0) [TNonce a]) -∗
+  pterm (TKey Dec k) ∨ pterm (TKey Dec k').
+Proof.
+iIntros "#meta"; iDestruct 1 as (a' k'') "# (meta' & pub & %e)".
+case/TExp_inj: e => _ /Permutation_singleton [] <-.
+by iPoseProof (meta_agree with "meta meta'") as "<-".
+Qed.
+
+Lemma nsl_dh_predX2 a k t :
+  nsl_dh_pred k (TExp (TInt 0) [TNonce a; t]) -∗
+  False.
+Proof.
+iDestruct 1 as (??) "# (_ & _ & %contra)".
+by case/TExp_inj: contra => _ /Permutation_length.
+Qed.
+
+Lemma pterm_dh1 a k k' :
+  nonce_pred a (nsl_dh_pred k) -∗
+  meta a (cryptoN.@"dh") k' -∗
+  pterm (TExp (TInt 0) [TNonce a])  ↔
+  ▷ (pterm (TKey Dec k) ∨ pterm (TKey Dec k')).
+Proof.
+iIntros "#a_pred #meta"; iSplit.
+- rewrite pterm_TExp1.
+  iDestruct 1 as "[[_ #contra] | #pub]".
+    rewrite pterm_TNonce.
+    iPoseProof (publishedE with "a_pred contra") as "{contra} contra".
+    iModIntro.
+    by iDestruct (nsl_dh_predN with "contra") as "[]".
+  rewrite nonces_of_term_eq /= left_id_L big_sepS_singleton.
+  iPoseProof (publishedE with "a_pred pub") as "{pub} pub".
+  by iModIntro; iApply nsl_dh_predX1; eauto.
+- iIntros "#pub".
+  rewrite pterm_TExp1 nonces_of_term_eq /= left_id_L; iRight.
+  rewrite big_sepS_singleton.
+  iApply (publishedE with "a_pred").
+  do 2!iModIntro.
+  by iExists a, k'; do 2!iSplit => //.
+Qed.
+
+Lemma pterm_dh2 a k t :
+  nonce_pred a (nsl_dh_pred k) -∗
+  pterm (TExp (TInt 0) [TNonce a; t]) -∗
+  ▷ pterm t.
+Proof.
+iIntros "#a_pred"; rewrite pterm_TExp2.
+iDestruct 1 as "# [[_ ?] | [ [_ contra] | pub]]"; eauto.
+- rewrite pterm_TNonce.
+  iPoseProof (publishedE with "a_pred contra") as "{contra} contra".
+  iModIntro.
+  by iDestruct (nsl_dh_predN with "contra") as "[]".
+- rewrite nonces_of_term_eq /= left_id_L big_sepS_union_pers.
+  rewrite big_sepS_singleton; iDestruct "pub" as "[pub _]".
+  iPoseProof (publishedE with "a_pred pub") as "{pub} pub".
+  iModIntro.
+  iDestruct (nsl_dh_predX2 with "pub") as "[]".
+Qed.
+
 Lemma wp_dh_initiator kA kB E Ψ :
   ↑cryptoN.@"nsl" ⊆ E →
   nsl_ctx nsl_dh_inv -∗
@@ -75,44 +147,26 @@ Lemma wp_dh_initiator kA kB E Ψ :
            □ (pterm gab → ▷ ▷ False))
        else True) -∗
       Ψ (repr ogab)) -∗
-  WP dh_initiator (TKey Dec kA) (TKey Enc kA) (TKey Enc kB) @ E
-     {{ Ψ }}.
+  WP dh_initiator (TKey Dec kA) (TKey Enc kA) (TKey Enc kB) @ E {{ Ψ }}.
 Proof.
 iIntros (?) "#ctx #? #? #? #p_e_kA #p_e_kB Hpost".
 rewrite /dh_initiator; wp_pures; wp_bind (mknonce _).
-iApply (wp_mknonce _ (λ t, (pterm (TKey Dec kA) ∨ pterm (TKey Dec kB)) ∧
-                           ∃ t', ⌜t = TExp (TInt 0) [t']⌝)%I).
+iApply (wp_mknonce _ (nsl_dh_pred kA)).
 iIntros (a) "#s_a #a_pred token".
+rewrite (meta_token_difference _ (↑cryptoN.@"dh")); last admit.
+iDestruct "token" as "[dh token]".
+iMod (meta_set _ _ kB with "dh") as "#dh"; eauto.
 wp_pures; wp_bind (tint _); iApply wp_tint.
 wp_pures; wp_bind (tgroup _); iApply wp_tgroup.
 wp_pures; wp_bind (texp _ _); iApply wp_texp.
 rewrite Spec.texpA; wp_pures; wp_bind (initiator _ _ _ _ _ _).
 iApply (wp_initiator with "ctx [] [] [] p_e_kA p_e_kB [] [] [] [token]") => //.
 - rewrite sterm_TExp sterm_TInt /=; eauto.
-- rewrite pterm_TExp1 pterm_TNonce; iModIntro; iSplit; last first.
-    iIntros "#pub"; iRight.
-    rewrite /= nonces_of_term_eq /= left_id_L.
-    by rewrite big_sepS_singleton; iApply publishedE; eauto.
-  iDestruct 1 as "[[_ pub] | pub]" => //.
-    by iPoseProof (publishedE with "a_pred pub") as "[??]"; eauto.
-  rewrite nonces_of_term_eq /= left_id_L big_sepS_singleton.
-  by iPoseProof (publishedE with "a_pred pub") as "{pub} #[pub ?]"; eauto.
+- by iModIntro; iApply pterm_dh1; eauto.
 - iIntros (nB); iRight; rewrite /=.
   iExists (TNonce a); iSplit => //.
-  iModIntro; iIntros (b).
-  rewrite pterm_TExp2.
-  iDestruct 1 as "# [[_ ?] | [[_ pub] | pub]]" => //.
-    rewrite pterm_TNonce.
-    iPoseProof (publishedE with "a_pred pub") as "{pub} pub"; iModIntro.
-    iDestruct "pub" as "[_ #pub]".
-    iDestruct "pub" as (t') "%e".
-    by rewrite unlock in e.
-  rewrite nonces_of_term_eq /= left_id_L big_sepS_union_pers.
-  iDestruct "pub" as "[pub _]".
-  rewrite big_sepS_singleton.
-  iPoseProof (publishedE with "a_pred pub") as "{pub} [? pub]"; iModIntro.
-  iDestruct "pub" as (t') "%e".
-  by case/TExp_inj: e => ? /Permutation_length.
+  iModIntro; iIntros (b) "p_b".
+  by iApply pterm_dh2.
 - rewrite /crypto_meta_token nonces_of_term_TExp /=.
   rewrite nonces_of_term_eq right_id_L left_id_L /=.
   iSplit; first by iPureIntro; set_solver.
@@ -138,9 +192,72 @@ iModIntro.
 rewrite pterm_TNonce.
 iPoseProof (publishedE with "a_pred succ") as "{contra} contra".
 iModIntro.
-iDestruct "contra" as "#[_ contra]".
-iDestruct "contra" as (?) "%e".
-by rewrite unlock in e.
+by iPoseProof (nsl_dh_predN with "contra") as "[]".
 Admitted.
 
-End NSL.
+Lemma wp_dh_responder kB E Ψ :
+  ↑cryptoN.@"nsl" ⊆ E →
+  nsl_ctx nsl_dh_inv -∗
+  crypto_enc (nroot.@"m1") msg1_pred -∗
+  crypto_enc (nroot.@"m2") msg2_pred -∗
+  crypto_enc (nroot.@"m3") msg3_pred -∗
+  pterm (TKey Enc kB) -∗
+  (∀ oresp : option (term * term),
+      (if oresp is Some (pkA, gab) then
+         ∃ kA,
+           ⌜pkA = TKey Enc kA⌝ ∧
+           pterm pkA ∧
+           sterm gab ∧
+           ((pterm (TKey Dec kA) ∨ pterm (TKey Dec kB)) ∨
+             □ (pterm gab → ▷ ▷ False))
+       else True) -∗
+      Ψ (repr oresp)) -∗
+  WP dh_responder (TKey Dec kB) (TKey Enc kB) @ E {{ Ψ }}.
+Proof.
+iIntros (?) "#ctx #? #? #? #p_e_kB Hpost".
+rewrite /dh_responder; wp_pures; wp_bind (mknonce _).
+iApply (wp_mknonce _ (nsl_dh_pred kB)).
+iIntros (b) "#s_b #b_pred token".
+rewrite (meta_token_difference _ (↑cryptoN.@"dh")); last admit.
+iDestruct "token" as "[dh token]".
+wp_pures; wp_bind (tint _); iApply wp_tint.
+wp_pures; wp_bind (tgroup _); iApply wp_tgroup.
+wp_pures; wp_bind (texp _ _); iApply wp_texp.
+rewrite Spec.texpA; wp_pures; wp_bind (responder _ _ _ _ _).
+iApply (wp_responder with "ctx [] [] [] p_e_kB [token] [] [dh]") => //.
+- rewrite /crypto_meta_token nonces_of_term_TExp /=.
+  rewrite nonces_of_term_eq right_id_L left_id_L /=.
+  iSplit; first by iPureIntro; set_solver.
+  rewrite big_sepS_singleton.
+  rewrite (meta_token_difference _ (↑cryptoN.@"nsl".@TExp (TInt 0) [TNonce b])).
+    by iDestruct "token" as "[??]".
+  admit.
+- rewrite sterm_TExp sterm_TInt /=; eauto.
+- iIntros (kA nA).
+  iMod (meta_set _ b kA with "dh") as "#meta"; eauto.
+  iModIntro; iSplit.
+  + by iModIntro; rewrite [(_ ∨ _)%I]comm; by iApply pterm_dh1.
+  + iExists (TNonce b); iSplit => //.
+    iIntros "!> %".
+    rewrite -[ [a; TNonce b]]/(seq.cat [a] [TNonce b]) TExpC /=.
+    by iIntros "#?"; iApply pterm_dh2.
+iIntros ([[pkA nA]|]) "resp"; last by protocol_failure.
+iDestruct "resp" as (kA) "# (-> & p_e_kA & s_nA & p_nA & inv)".
+wp_pures; wp_bind (texp _ _); iApply wp_texp; wp_pures.
+iApply ("Hpost" $! (Some (TKey Enc kA, Spec.texp nA (TNonce b)))).
+iExists _; do 3!iSplit => //; eauto.
+  by iApply sterm_texp.
+iDestruct "inv" as "[inv|inv]"; eauto.
+iDestruct "inv" as (t) "[-> #inv]".
+rewrite Spec.texpA.
+rewrite -[ [TNonce b; t]]/(seq.cat [TNonce b] [t]) TExpC /=.
+iRight; iIntros "!> #contra".
+iSpecialize ("inv" with "contra").
+iModIntro.
+rewrite pterm_TNonce.
+iPoseProof (publishedE with "b_pred inv") as "{inv} inv".
+iModIntro.
+by iDestruct (nsl_dh_predN with "inv") as "[]".
+Admitted.
+
+End NSLDH.
